We have two base cases: $~i = 0~$ and $~i = 1~$. For $~i = 0~$ , we have

$$
\begin{align*}
\frac{\phi^0 - \hat{\phi}^0}{\sqrt{5}}
&= \frac{1 - 1}{\sqrt{5}} \\
&= 0 \\
&= F_0,
\end{align*}
$$

and for $~i = 1~$ , we have

$$
\begin{align*}
\frac{\phi^1 - \hat{\phi}^1}{\sqrt{5}}
&= \frac{(1 + \sqrt{5}) - (1 - \sqrt{5})}{2\sqrt{5}} \\
&= \frac{2\sqrt{5}}{2\sqrt{5}} \\
&= 1 \\
&= F_1.
\end{align*}
$$

For the inductive case, the inductive hypothesis is that $~F_{i-1} = (\phi^{i-1} - \hat{\phi}^{i-1})/\sqrt{5}$ and $F_{i-2} = (\phi^{i-2} - \hat{\phi}^{i-2})/\sqrt{5}$ . We have

$$
\begin{align*}
F_i
&= F_{i-1} + F_{i-2} && (\text{equation } \mathit{Fibonacci}) \\
&= \frac{\phi^{i-1} - \hat{\phi}^{i-1}}{\sqrt{5}} + \frac{\phi^{i-2} - \hat{\phi}^{i-2}}{\sqrt{5}} && \text{(inductive hypothesis)} \\
&= \frac{\phi^{i-2}(\phi + 1) - \hat{\phi}^{i-2}(\hat{\phi} + 1)}{\sqrt{5}} \\
&= \frac{\phi^{i-2}\phi^2 - \hat{\phi}^{i-2}\hat{\phi}^2}{\sqrt{5}} && (\text{definition of }\phi) \\
&= \frac{\phi^i - \hat{\phi}^i}{\sqrt{5}}.
\end{align*}
$$
